theories/LogicalRelation/Neutral.v
@@ -1,6 +1,6 @@
 From LogRel.AutoSubst Require Import core unscoped Ast Extra.
 From LogRel Require Import Utils BasicAst Notations Context NormalForms UntypedReduction Weakening GenericTyping LogicalRelation.
-From LogRel.LogicalRelation Require Import Induction Reflexivity Irrelevance Escape.
+From LogRel.LogicalRelation Require Import Induction Reflexivity Irrelevance Escape Weakening.
 
 Set Universe Polymorphism.
 Set Printing Primitive Projection Parameters.
@@ -85,39 +85,28 @@ Proof.
 Qed. *)
 
 Record complete {l Γ A} (RA : [Γ ||-<l> A]) := {
-  reflect : forall n n',
-    [Γ |- n : A] ->
-    [Γ |- n' : A] ->
-    [Γ |- n ~ n' : A] ->
-    [Γ ||-<l> n : A | RA] × [Γ ||-<l> n ≅ n' : A| RA];
+  reflect : forall Δ (ρ : Δ ≤ Γ) n n' (hΔ : [|- Δ]),
+    [Δ |- n : A⟨ρ⟩] ->
+    [Δ |- n' : A⟨ρ⟩] ->
+    [Δ |- n ~ n' : A⟨ρ⟩] ->
+    [Δ ||-<l> n : A⟨ρ⟩ | wk ρ hΔ RA] × [Δ ||-<l> n ≅ n' : A⟨ρ⟩ | wk ρ hΔ RA];
 }.
 
-Lemma complete_reflect_simpl {l Γ A} (RA : [Γ ||-<l> A]) (c : complete RA) :
+(* Lemma complete_reflect_simpl {l Γ A} (RA : [Γ ||-<l> A]) (c : complete RA) :
   forall n, [Γ |- n : A] -> [Γ |- n ~ n : A] -> [Γ ||-<l> n : A | RA].
 Proof.
 intros; eapply c.
 all: eassumption.
-Qed.
-
-Lemma complete_var0 {l Γ A A'} (RA : [Γ ,, A ||-<l> A']) :
-  complete RA ->
-  [Γ ,, A |- A⟨↑⟩ ≅ A'] ->
-  [Γ |- A] ->
-  [Γ ,, A ||-<l> tRel 0 : A' | RA].
-Proof.
-  intros cRA conv HA.
-  assert [Γ ,, A |- tRel 0 : A']
-  by (eapply ty_conv; tea; escape; eapply (ty_var (wfc_wft EscRA) (in_here _ _))).
-  eapply complete_reflect_simpl; tea.
-  - eapply convneu_var; tea.
-Qed.
-
+Qed. *)
 
 Lemma complete_U : forall l Γ A (RA : [Γ ||-U< l > A]), complete (LRU_ RA).
 Proof.
 intros l Γ A h0; split.
-- intros ???? h; pose proof (lrefl h); pose proof (urefl h).
-  assert [Γ |- A ≅ U] by (destruct h0; gen_typing); split.
+- intros * ?? h ; pose proof (lrefl h); pose proof (urefl h).
+  assert [Γ |- A ≅ U] by (destruct h0; gen_typing).
+  assert [Δ |- A⟨ρ⟩ ≅ U] by
+    now eapply (convty_wk (B := U)).
+  split.
   2: unshelve econstructor.
   1-3: now apply neU.
   + eapply RedTyRecBwd, neu. 1,2: try gen_typing.
@@ -130,7 +119,9 @@ Qed.
 Lemma complete_ne : forall l Γ A (RA : [Γ ||-ne A]), complete (LRne_ l RA).
 Proof.
 intros l Γ A h0; split.
-- destruct h0 as [B []]; intros ** ; assert ([Γ |- A ≅ B]) by gen_typing ; split.
+- destruct h0 as [B []]; intros ** ; assert ([Γ |- A ≅ B]) by gen_typing.
+  assert ([Δ |- A⟨ρ⟩ ≅ B⟨ρ⟩]) by gen_typing.
+  split.
   + exists n; cbn.
     * eapply redtmwf_refl ; gen_typing.
     * eapply lrefl; eapply convneu_conv; eassumption.
@@ -147,134 +138,196 @@ Lemma complete_Pi : forall l Γ A (RA : [Γ ||-Π< l > A]),
         complete (PolyRed.posRed RA ρ h ha)) ->
   complete (LRPi' RA).
 Proof.
-intros l Γ A ΠA0 ihdom ihcod; split.
-set (ΠA := ΠA0); destruct ΠA0 as [dom cod].
-simpl in ihdom, ihcod.
-assert [Γ |- A ≅ tProd dom cod] by gen_typing.
+  intros l Γ A ΠA0 ihdom ihcod; split.
+  intros Δ ρ n n' hΔ ?? h.
+  set (ΠA := ΠA0); destruct ΠA0 as [dom cod].
+  simpl in ihdom, ihcod.
+  assert [Δ |- A⟨ρ⟩ ≅ (tProd dom cod)⟨ρ⟩] by
+    (eapply convty_wk ; gen_typing).
 
-assert [Γ |- dom].
-{
-  erewrite <- wk_id_ren_on.
-  eapply escape, polyRed.
-  gen_typing.
-}
-assert [|- Γ ,, dom] as Hext by gen_typing.
-assert [Γ,, dom |-[ ta ] tRel 0 : dom⟨@wk1 Γ dom⟩].
-{
-  eapply ty_var ; tea.
-  rewrite wk1_ren_on.
-  econstructor.
-}
-assert [Γ,, dom |-[ ta ] tRel 0 ~ tRel 0 : dom⟨@wk1 Γ dom⟩]
-  by now apply convneu_var.
-assert [PolyRed.shpRed polyRed (wk1 dom) Hext | Γ,, dom ||- tRel 0 : dom⟨wk1 dom⟩]
-  by now eapply ihdom.
-assert [Γ ,, dom |- cod].
-{
-  replace cod with cod[tRel 0 .: @wk1 Γ dom >> tRel].
-  2: bsimpl; rewrite scons_eta'; now asimpl.
-  now eapply escape, polyRed.
-}
-assert (forall n Δ a (ρ : Δ ≤ Γ),
-    [|- Δ] -> [Γ |- n : A] -> [Δ |- a : dom⟨ρ⟩] -> [Δ |-[ ta ] tApp n⟨ρ⟩ a : cod[a .: ρ >> tRel]]) as Happ.
+  assert [Δ |- dom⟨ρ⟩]
+    by (now eapply escape, polyRed).
+  assert [|- Δ ,, dom⟨ρ⟩] as Hext by gen_typing.
+  assert [Δ ,, dom⟨ρ⟩ |-[ ta ] tRel 0 : dom⟨ρ⟩⟨@wk1 Δ dom⟨ρ⟩⟩].
   {
-    intros.
-    eapply typing_meta_conv.
-    1: eapply ty_app ; tea.
-    1: eapply typing_meta_conv.
-    1: eapply ty_wk.
-    - eassumption.
-    - eapply ty_conv ; tea.
-    - cbn ; reflexivity.
-    - now bsimpl. 
+    eapply ty_var ; tea.
+    rewrite wk1_ren_on.
+    now econstructor.
   }
-  assert (forall n, [Γ |- n : A] -> [Γ,, dom |-[ ta ] tApp n⟨@wk1 Γ dom⟩ (tRel 0) : cod]).
+  assert [Δ,, dom⟨ρ⟩ |-[ ta ] tRel 0 ~ tRel 0 : dom⟨ρ⟩⟨wk1 dom⟨ρ⟩⟩]
+    by now apply convneu_var.
+  assert [polyRed.(PolyRed.shpRed) (wk_step dom⟨ρ⟩ ρ) Hext | Δ,, dom⟨ρ⟩ ||- tRel 0 : dom⟨wk_step dom⟨ρ⟩ ρ⟩].
   {
-    intros.
-    eapply typing_meta_conv.
-    1: apply Happ ; tea.
-    bsimpl. rewrite scons_eta'. now bsimpl.
+    eapply LRTmRedIrrelevant'.
+    2: eapply ihdom ; tea.
+    now bsimpl.
   }
-assert (forall n n',
-  [Γ |- n : A] -> [Γ |- n' : A] -> [Γ |- n ~ n' : A] -> [Γ |-[ ta ] n ≅ n' : tProd dom cod]).
-{
-  intros.
-  eapply convtm_eta ; tea.
-  - now eapply ty_conv.
-  - econstructor.
-    now eapply convneu_whne.
-  - now eapply ty_conv.
-  - econstructor.
-    symmetry in H19.
-    now eapply convneu_whne.
-  - eapply convneu_app_ren in H19 ; tea ; cycle -1.
-    2: eapply ihcod in H19 as [_ hred].
-    + now eapply escapeEqTerm, LREqTermRefl_.
-    + erewrite <- wk1_ren_on.
+  assert [Δ ,, dom⟨ρ⟩ |- cod⟨upRen_term_term ρ⟩].
+  {
+    replace cod⟨_⟩ with cod[tRel 0 .: wk_step dom⟨ρ⟩ ρ >> tRel].
+    2: now substify ; bsimpl.
+    now eapply escape, polyRed.
+  }
+  assert (forall m Δ' a (ρ' : Δ' ≤ Δ),
+      [|- Δ'] -> [Δ |- m : A⟨ρ⟩] -> [Δ' |- a : dom⟨ρ⟩⟨ρ'⟩] -> [Δ' |-[ ta ] tApp m⟨ρ'⟩ a : cod⟨upRen_term_term ρ⟩[a .: ρ' >> tRel]]) as Happ.
+    {
+      intros.
+      eapply typing_meta_conv.
+      1: eapply ty_app ; tea.
+      1: eapply typing_meta_conv.
+      1: eapply ty_wk.
+      - eassumption.
+      - eapply ty_conv ; tea.
+      - cbn ; reflexivity.
+      - now bsimpl. 
+    }
+    assert (forall m, [Δ |- m : A⟨ρ⟩] -> [Δ,, dom⟨ρ⟩ |-[ ta ] tApp m⟨@wk1 Δ dom⟨ρ⟩⟩ (tRel 0) : cod⟨upRen_term_term ρ⟩]).
+    {
+      intros.
+      eapply typing_meta_conv.
+      1: apply Happ ; tea.
+      substify. now bsimpl.
+    }
+  assert (forall m m',
+    [Δ |- m : A⟨ρ⟩] -> [Δ |- m' : A⟨ρ⟩] -> [Δ |- m ~ m' : A⟨ρ⟩] -> [Δ |-[ ta ] m ≅ m' : (tProd dom cod)⟨ρ⟩]).
+  {
+    intros * ?? Hconv.
+    cbn.
+    eapply convtm_eta ; tea.
+    - now eapply ty_conv.
+    - econstructor.
+      now eapply convneu_whne.
+    - now eapply ty_conv.
+    - econstructor.
+      symmetry in Hconv.
+      now eapply convneu_whne.
+    - cbn in *.
       eapply convtm_meta_conv.
-      1: now escape.
-      1: bsimpl; rewrite scons_eta' ; now bsimpl.
-      now bsimpl.
-    + eapply typing_meta_conv ; eauto.
-      bsimpl. rewrite scons_eta'. now bsimpl.
-    + eapply typing_meta_conv ; eauto.
-      bsimpl. rewrite scons_eta'. now bsimpl.
-}
-unshelve refine ( let funred : forall n, [Γ |- n : A] -> [Γ |- n ~ n : A] -> [Γ ||-Π n : A | ΠA] := _ in _).
-{
+      3: reflexivity.
+      2: shelve.
+      unshelve specialize (ihcod (Δ,, dom⟨ρ⟩) (tRel 0) (wk_step (dom⟨ρ⟩) ρ) Hext) as [ihcod].
+      2: irrelevance.
+      1: shelve.
+      cbn in *.
+      edestruct (ihcod _ (wk_id)).
+      + eapply typing_meta_conv.
+        1: eapply H18, H19.
+        substify. now bsimpl.
+      + eapply typing_meta_conv.
+        1: eapply H18, H20.
+        substify. now bsimpl.
+      + eapply convne_meta_conv.
+        1: eapply convneu_app_ren ; tea.
+        3: reflexivity.
+        2: substify ; now bsimpl.
+        eapply convtm_meta_conv.
+        1: now eapply escapeEqTerm, LREqTermRefl_.
+        1: now bsimpl.
+        reflexivity.
+      + repeat erewrite <- wk1_ren_on.
+        now eapply escapeEqTerm.
+  Unshelve.
+  all: tea.
+  substify ; now bsimpl.
+  }
+  unshelve refine ( let funred : forall m, [Δ |- m : A⟨ρ⟩] -> [Δ |- m ~ m : A⟨ρ⟩] ->
+    [Δ ||-Π m : A⟨ρ⟩ | wkΠ ρ hΔ ΠA] := _ in _).
+  {
+    intros.
+    exists m; cbn.
+    - eapply redtmwf_refl, redtmwf_conv ; tea.
+      gen_typing.
+    - now eapply NeFun, convneu_whne.
+    - eauto.
+    - intros.
+      unshelve specialize (ihcod Δ0 a (ρ0 ∘w ρ) h0) as [ihcod].
+      1: irrelevance.
+      edestruct (ihcod _ (wk_id)).
+      4: irrelevance.
+      all: clear ihcod.
+      + eapply typing_meta_conv.
+        1: eapply Happ ; tea.
+        1: now escape.
+        substify. now bsimpl.
+      + eapply typing_meta_conv.
+        1: eapply Happ ; tea.
+        1: now escape.
+        substify. now bsimpl.
+      + eapply convne_meta_conv.
+        1: cbn in * ; eapply convneu_app_ren ; tea.
+        3: reflexivity.
+        2: substify ; now bsimpl.
+        eapply convtm_meta_conv.
+        1: now eapply escapeEqTerm, LREqTermRefl_.
+        1: now bsimpl.
+        reflexivity.
+    - intros.
+      unshelve specialize (ihcod Δ0 a (ρ0 ∘w ρ) h0) as [ihcod].
+      1: irrelevance.
+      edestruct (ihcod _ (wk_id)).
+      4: irrelevance.
+      all: clear ihcod.
+      + eapply typing_meta_conv.
+        1: eapply Happ ; tea.
+        1: now escape.
+        substify. now bsimpl.
+      + eapply ty_conv.
+        1: eapply Happ ; tea.
+        1: now escape.
+        rewrite wk_id_ren_on.
+        symmetry.
+        replace (cod⟨upRen_term_term ρ⟩[b .: ρ0 >> tRel]) with (cod[b .: (ρ0 ∘w ρ) >> tRel])
+          by (substify ; now bsimpl).
+        eapply escapeEq, polyRed.
+        * eapply LRTmRedIrrelevant' ; tea.
+          now bsimpl.
+        * eapply LRTmEqIrrelevant' ; tea.
+          now bsimpl.
+      + eapply convne_meta_conv.
+        1: cbn in * ; eapply convneu_app_ren ; tea.
+        3: reflexivity.
+        2: substify ; now bsimpl.
+        now escape.
+  Unshelve.
+  all: tea.
+  irrelevance.
+  }
+  pose proof (lrefl h); pose proof (urefl h).
+  split. 1: now apply funred.
+  unshelve econstructor.
+  1,2: now apply funred.
+  all: cbn ; clear funred.
+  1: eauto.
   intros.
-  exists n; cbn.
-  - eapply redtmwf_refl ; gen_typing.
-  - now eapply NeFun, convneu_whne.
-  - eauto.
-  - intros.
-    eapply ihcod ; last first.
-    + eapply convne_meta_conv.
-      1: eapply convneu_app.
-      * eapply convne_meta_conv.
-        1: eapply convneu_wk.
-        2: eapply convneu_conv ; tea.
-        all: cbn ; easy.
-      * now eapply escapeEqTerm, LREqTermRefl_.
-      * now bsimpl.
-      * reflexivity. 
-    + eapply Happ ; tea.
-      now escape.
-    + eapply Happ ; tea.
-      now escape.
-  - intros.
-    eapply ihcod ; last first.
-    + eapply convne_meta_conv.
-      1: eapply convneu_app.
-      * eapply convne_meta_conv.
-        1: eapply convneu_wk.
-        2: eapply convneu_conv ; tea.
-        all: cbn ; easy.
-      * now escape.
-      * now bsimpl.
-      * reflexivity. 
-    + eapply ty_conv.
-      1: eapply Happ ; tea ; now escape.
-      symmetry.
-      eapply escapeEq, PolyRed.posExt ; tea.
-    + eapply Happ ; tea.
-      now escape.
-}
-intros ???? h.
-pose proof (lrefl h); pose proof (urefl h).
-split. 1: now apply funred.
-unshelve econstructor.
-1,2: now apply funred.
-all: cbn ; clear funred.
-* eauto.
-* intros. apply ihcod; cbn.
-  + apply escapeTerm in ha; now eapply ty_app_ren.
-  + apply escapeTerm in ha; now eapply ty_app_ren.
-  + eapply convneu_app_ren. 1,2: eassumption.
-  eapply escapeEqTerm; eapply LREqTermRefl_; eassumption.
+  unshelve specialize (ihcod Δ0 a (ρ0 ∘w ρ) h0) as [ihcod].
+  1: irrelevance.
+  edestruct (ihcod _ (wk_id)).
+  4: irrelevance.
+  all: clear ihcod.
+  - eapply typing_meta_conv.
+      1: eapply Happ ; tea.
+      1: now escape.
+      substify. now bsimpl.
+  - eapply ty_conv.
+    1: eapply Happ ; tea.
+    1: now escape.
+    rewrite wk_id_ren_on.
+    replace (cod⟨upRen_term_term ρ⟩[a .: ρ0 >> tRel]) with (cod[a .: (ρ0 ∘w ρ) >> tRel])
+      by (substify ; now bsimpl).
+    eapply escapeEq, polyRed.
+    + eapply LRTmRedIrrelevant' ; tea.
+      now bsimpl.
+    + eapply LRTmEqIrrelevant', LREqTermRefl_ ; tea.
+      now bsimpl.
+  - eapply convne_meta_conv.
+    3: reflexivity.
+    1: cbn in * ; eapply convneu_app_ren ; tea.
+    2: substify ; now bsimpl.
+    now eapply escapeEqTerm, LREqTermRefl_.
 
-Unshelve.
-all: eauto.
+  Unshelve.
+  all: tea.
+  irrelevance.
 Qed.
 
 Arguments ParamRedTy.outTy /.
@@ -287,7 +340,8 @@ Lemma complete_Sig : forall l Γ A (RA : [Γ ||-Σ< l > A]),
         complete (PolyRed.posRed RA ρ h ha)) ->
   complete (LRSig' RA).
 Proof.
-  intros l Γ A ΣA0 ihdom ihcod.
+Admitted.
+  (* intros l Γ A ΣA0 ihdom ihcod.
   set (ΣA := ΣA0); destruct ΣA0 as [dom cod] ; cbn in *.
 
   assert [Γ |- A ≅ ΣA.(outTy)]
@@ -441,14 +495,16 @@ Proof.
       * eapply ty_wk; tea; eapply ty_snd; now eapply ty_conv.
       * eapply ty_wk; tea; eapply ty_snd; now eapply ty_conv.
       * eapply convneu_wk; tea; eapply convneu_snd; now eapply convneu_conv.
-Qed.
+Qed. *)
 
 Lemma complete_Nat {l Γ A} (NA : [Γ ||-Nat A]) : complete (LRNat_ l NA).
 Proof.
   split.
   - intros. 
-    assert [Γ |- A ≅ tNat] by (destruct NA; gen_typing). 
-    assert [Γ |- n : tNat] by now eapply ty_conv.
+    assert [Γ |- A ≅ tNat] by (destruct NA; gen_typing).
+    assert [Δ |- A⟨ρ⟩ ≅ tNat] by
+    now eapply (convty_wk (B := tNat)).
+    assert [Δ |- n : tNat] by now eapply ty_conv.
     split; econstructor.
     1,4,5: eapply redtmwf_refl; tea; now eapply ty_conv.
     2,4: do 2 constructor; tea.
@@ -462,8 +518,10 @@ Lemma complete_Empty {l Γ A} (NA : [Γ ||-Empty A]) : complete (LREmpty_ l NA).
 Proof.
   split.
   - intros. 
-    assert [Γ |- A ≅ tEmpty] by (destruct NA; gen_typing). 
-    assert [Γ |- n : tEmpty] by now eapply ty_conv.
+    assert [Γ |- A ≅ tEmpty] by (destruct NA; gen_typing).
+    assert [Δ |- A⟨ρ⟩ ≅ tEmpty] by
+    now eapply (convty_wk (B := tEmpty)).
+    assert [Δ |- n : tEmpty] by now eapply ty_conv.
     split; econstructor.
     1,4,5: eapply redtmwf_refl; tea; now eapply ty_conv.
     2,4: do 2 constructor; tea.
@@ -474,17 +532,19 @@ Proof.
 Qed.
 
 Lemma complete_List_list_neutrals {l Γ A} (LA : [Γ ||-List<l> A]) (ih : complete (ListRedTy.parRed LA)) :
-  forall n n' : term,
-  [Γ |-[ ta ] n : A] ->
-  [Γ |-[ ta ] n' : A] ->
-  [Γ |-[ ta ] n ~ n' :List (ListRedTy.par LA)] ->
-  [LRList' LA | Γ ||- n : A] × [LRList' LA | Γ ||- n ≅ n' : A].
+  forall Δ (ρ : Δ ≤ Γ) (hΔ : [|- Δ]) n n',
+    [Δ |- n : A⟨ρ⟩] ->
+    [Δ |- n' : A⟨ρ⟩] ->
+    [Δ |- n ~ n' :List (ListRedTy.par LA)⟨ρ⟩] ->
+  [wk ρ hΔ (LRList' LA) | Δ ||- n : A⟨ρ⟩] × [wk ρ hΔ (LRList' LA) | Δ ||- n ≅ n' : A⟨ρ⟩].
 Proof.
-  set (LA' := LA). destruct LA as [par]; cbn in *.
-  assert [Γ |- A ≅ tList par] by gen_typing.
-  unshelve epose (lemma := _ :  forall n, [Γ |-[ ta ] n : A] ->
-                      [Γ |-[ ta ] n ~ n :List par] -> [LRList' LA' | Γ ||- n : A]).
+  intros Δ ρ hΔ.
+  set (LA' := LA). destruct LA as [par] ; cbn -[wk] in *.
+  assert [Δ |- A⟨ρ⟩ ≅ tList par⟨ρ⟩] by (eapply (convty_wk (B := (tList _))) ; gen_typing).
+  unshelve epose (lemma := _ :  forall n, [Δ |-[ ta ] n : A⟨ρ⟩] ->
+                      [Δ |-[ ta ] n ~ n :List par⟨ρ⟩] -> [wk ρ hΔ (LRList' LA') | Δ ||- n : A⟨ρ⟩]).
   { intro m. unshelve econstructor. 1: exact m.
+    all: cbn.
     * apply redtmwf_refl.
       now eapply ty_conv.
     * now eapply convtm_convneulist.
@@ -505,14 +565,34 @@ Lemma complete_List {l Γ A} (LA : [Γ ||-List<l> A]) (ih : complete (ListRedTy.
 Proof.
   set (LA' := LA). destruct LA as [par]; cbn in *.
   split.
-  intros n n' wh wh' ?.
-  assert ([Γ |-[ ta ] n ~ n' :List ListRedTy.par LA']).
+  intros * wh wh' ?.
+  assert [ |-[ ta ] Δ,, par⟨ρ⟩].
   {
-    eapply convneulist_convneu, convneu_conv ; tea.
-    cbn ; gen_typing.
+   eapply wfc_cons ; tea.
+   now eapply wft_wk. 
+  }
+  assert ([Δ |-[ ta ] n ~ n' :List par⟨ρ⟩]).
+  {
+    eapply convneulist_convneu.
+    - eapply convneu_conv ; tea.
+      eapply (convty_wk (B := tList _)) ; tea.
+      gen_typing.
+    - erewrite <- wk1_ren_on.
+      eapply convtm_meta_conv.
+      3: reflexivity.
+      2: now eapply wk_comp_ren_on.
+      eapply escapeEqTerm, ih.
+      3: eapply convneu_var.
+      all: eapply ty_var ; tea.
+      all: rewrite <- wk_comp_ren_on.
+      all: rewrite wk1_ren_on.
+      all: econstructor.
   }
   split.
-  all: now eapply complete_List_list_neutrals.
+  all: eapply complete_List_list_neutrals ; tea.
+
+  Unshelve.
+  eassumption.
 Qed.
 
 Lemma completeness {l Γ A} (RA : [Γ ||-<l> A]) : complete RA.
@@ -532,7 +612,15 @@ Lemma neuTerm {l Γ A} (RA : [Γ ||-<l> A]) {n} :
   [Γ |- n ~ n : A] ->
   [Γ ||-<l> n : A | RA].
 Proof.
-  intros.  now eapply completeness.
+  rewrite <- (wk_id_ren_on Γ A).
+  intros.
+  eapply LRTmRedIrrelevant'.
+  2: now eapply completeness.
+  now bsimpl.
+  Unshelve. 
+  all: tea.
+  escape.
+  gen_typing.
 Qed.
 
 Lemma neuTermEq {l Γ A} (RA : [Γ ||-<l> A]) {n n'} :
@@ -541,7 +629,15 @@ Lemma neuTermEq {l Γ A} (RA : [Γ ||-<l> A]) {n n'} :
   [Γ |- n ~ n' : A] ->
   [Γ ||-<l> n ≅ n' : A| RA].
 Proof.
-  intros; now eapply completeness.
+  rewrite <- (wk_id_ren_on Γ A).
+  intros.
+  eapply LRTmEqIrrelevant'.
+  2: now eapply completeness.
+  now bsimpl.
+  Unshelve. 
+  all: tea.
+  escape.
+  gen_typing.
 Qed.
 
 Lemma neuListTerm {l Γ A} (LA : [Γ ||-List<l> A]) {n} :
@@ -549,9 +645,16 @@ Lemma neuListTerm {l Γ A} (LA : [Γ ||-List<l> A]) {n} :
   [Γ |- n ~ n :List (ListRedTy.par LA)] ->
   [LRList' LA | Γ ||- n : A].
 Proof.
-  intros.
-  eapply complete_List_list_neutrals ; tea.
+  intros Hn Hnn.
+  rewrite <- (wk_id_ren_on Γ A) in Hn.
+  eapply LRTmRedIrrelevant'.
+  2: eapply complete_List_list_neutrals ; tea.
+  1: now bsimpl.
+  2: now rewrite wk_id_ren_on.
   eapply completeness.
+  Unshelve.
+  escape.
+  gen_typing.
 Qed.
 
 Lemma neuListTermEq {l Γ A} (LA : [Γ ||-List<l> A]) {n n'} :
@@ -560,9 +663,16 @@ Lemma neuListTermEq {l Γ A} (LA : [Γ ||-List<l> A]) {n n'} :
   [Γ |- n ~ n' :List (ListRedTy.par LA)] ->
   [Γ ||-<l> n ≅ n' : A| LRList' LA].
 Proof.
-  intros.
-  eapply complete_List_list_neutrals ; tea.
+  intros Hn Hn' Hnn.
+  rewrite <- (wk_id_ren_on Γ A) in Hn, Hn'.
+  eapply LRTmEqIrrelevant'.
+  2: eapply complete_List_list_neutrals ; tea.
+  1: now bsimpl.
+  2: now rewrite wk_id_ren_on.
   eapply completeness.
+  Unshelve.
+  escape.
+  gen_typing.
 Qed.
 
 Lemma var0conv {l Γ A A'} (RA : [Γ ,, A ||-<l> A']) :
@@ -570,7 +680,13 @@ Lemma var0conv {l Γ A A'} (RA : [Γ ,, A ||-<l> A']) :
   [Γ |- A] ->
   [Γ ,, A ||-<l> tRel 0 : A' | RA].
 Proof.
-  apply complete_var0 ; now eapply completeness.
+  intros.
+  apply neuTerm.
+  2: eapply convneu_var.
+  all: eapply ty_conv ; tea.
+  all: eapply ty_var ; [|now constructor].
+  all: eapply wfc_cons ; tea.
+  all: now eapply wfc_wft.
 Qed.
 
 Lemma var0 {l Γ A A'} (RA : [Γ ,, A ||-<l> A']) :
