theories/Context.v
@@ -1,5 +1,5 @@
 (** * LogRel.Context: definition of contexts and operations on them.*)
-From Coq Require Import ssreflect Morphisms Setoid.
+From Coq Require Import ssreflect Morphisms Setoid List.
 From LogRel.AutoSubst Require Import core unscoped Ast Extra.
 From LogRel Require Import Utils BasicAst.
 
